add if etc

Judge.v
@@ -10,7 +10,7 @@ Require Import ListSet.
 Require Import Subst.
 Require Import Translation.
  
-Reserved Notation "P / G ⊢ s ::: O " (at level 0, no associativity).
+Reserved Notation "( Φ ; Γ ; Ξ ) ⊢ s ::: O" (at level 0, no associativity).
 
 Definition wf_subst θ := forall v, θ v = ν <-> v = ν.
 
@@ -70,6 +70,12 @@ Inductive wf_env : type_env -> Prop :=
 (* ------------------------------------------------------------------- *)
     wf_env ((x, T) :: Γ).
 
+Definition wf_guard (Γ : type_env) (ξ : guard) :=
+  wf_prop Γ ξ /\ ~(ν ∈ fv_prop ξ).
+
+Definition wf_guards (Γ : type_env) (Ξ : guards) :=
+  Forall (fun ξ => wf_guard Γ ξ) Ξ.
+
 Inductive wf_schema : proc_schema -> Prop :=
 | wf_proc_schema : 
     forall S, 
@@ -80,46 +86,49 @@ Inductive wf_schema : proc_schema -> Prop :=
 (* ------------------------------------------------------------------- *)
   wf_schema S.
 
-Inductive subtype : type_env -> reft_type -> reft_type -> Prop :=
-| st_base : forall Γ b p p',
-             ((sep_env Γ) |-- (sep_pred p --> sep_pred p')) ->
+Inductive subtype : type_env -> guards -> reft_type -> reft_type -> Prop :=
+| st_base : 
+    forall Γ Ξ b p p',
+      ((sep_env Γ && sep_guards Ξ) |-- (sep_pred p --> sep_pred p')) ->
 (* ------------------------------------------------------------------- *)
-  subtype Γ { ν : b | p } { ν : b | p' }.
+  subtype Γ Ξ { ν : b | p } { ν : b | p' }.
 
-Inductive expr_type : type_env -> expr -> reft_type -> Prop :=
-| t_const : forall Γ v,
+Inductive expr_type : type_env -> guards -> expr -> reft_type -> Prop :=
+| t_const : forall Γ Ξ v,
 (* ------------------------------------------------------------------- *)
-  expr_type Γ (value_e v) { ν : (base_of_val v) | (var_e ν) .= (value_e v) }
+  expr_type Γ Ξ (value_e v) { ν : (base_of_val v) | (var_e ν) .= (value_e v) }
             
-| t_var : forall Γ x τ φ, (x, { ν : τ | φ }) ∈ Γ ->
+| t_var : forall Γ Ξ x τ φ, (x, { ν : τ | φ }) ∈ Γ ->
 (* ------------------------------------------------------------------- *)
-  expr_type Γ (var_e x) { ν : τ | φ }
+  expr_type Γ Ξ (var_e x) { ν : τ | φ }
 
-| t_sub : forall Γ e T T',
-            expr_type Γ e T -> wf_type Γ T' -> subtype Γ T T' -> 
+| t_sub : forall Γ Ξ e T T',
+            expr_type Γ Ξ e T -> wf_type Γ T' -> subtype Γ Ξ T T' -> 
 (* ------------------------------------------------------------------- *)
-  expr_type Γ e T'.
+  expr_type Γ Ξ e T'.
 
-Definition tc_list Γ (xts : list (var * reft_type)) :=
+Definition tc_list Γ Ξ (xts : list (var * reft_type)) :=
   Forall (fun xt => 
-            expr_type Γ (var_e (fst xt)) (snd xt)) xts.
+            expr_type Γ Ξ (var_e (fst xt)) (snd xt)) xts.
 
-Fixpoint subst_of_list (sub : list (var*var)) : subst_t var var :=
-  fun i => 
-    match sub with
-      | (x,x') :: sub' => if eq_dec i x then x' else subst_of_list sub' i
-      | _ => i
-    end.
+Definition join_var Ξ Γ1 Γ2 xt :=
+  match xt with
+  | (x, t) =>
+    (exists t1, ((x,t1) ∈ Γ1 /\ subtype Γ1 Ξ t1 t))
+    /\ (exists t2, ((x,t2) ∈ Γ1 /\ subtype Γ2 Ξ t2 t))
+  end.
 
-Definition subst_call S (xr : var) (xs : list var) := 
-  subst_of_list ((fst (s_ret S), xr) :: (combine (s_formals S) xs)).
+Definition join_env Ξ Γ1 Γ2 Γ :=
+  Forall (fun xt => xt ∈ Γ /\ wf_type Γ (snd xt) /\ join_var Ξ Γ1 Γ2 xt) Γ.
+  
                               
-Inductive stmt_type : proc_env -> type_env -> stmt -> type_env -> Prop :=
-| t_skip : forall Φ Γ,
+Inductive stmt_type : proc_env -> type_env -> guards -> stmt -> type_env -> Prop :=
+| t_skip : forall Φ Γ Ξ,
 (* ------------------------------------------------------------------- *)
-  (Φ / Γ ⊢ skip_s ::: Γ)
+   (Φ ; Γ ; Ξ) ⊢ skip_s ::: Γ
+
 | t_proc_s : 
-    forall Φ Γ (v:var) f p S xs ts θ θS,
+    forall Φ Γ Ξ (v:var) f p S xs ts θ θS,
       (f,(p,S)) ∈ Φ -> wf_schema S -> wf_subst θ ->
       θS = subst θ S ->
       xs = subst θ (s_formals S) ->
@@ -129,17 +138,27 @@ Inductive stmt_type : proc_env -> type_env -> stmt -> type_env -> Prop :=
       (forall x', ~(In x' (fst (s_ret S) :: s_formals S)) -> θ x' = x') ->
       wf_env (subst θ (s_ret S) :: Γ) ->
       Forall (fun t => wf_type Γ t) ts ->
-      tc_list Γ (combine xs ts) ->
+      tc_list Γ Ξ (combine xs ts) ->
 (* ------------------------------------------------------------------- *)
-  (Φ / Γ ⊢ proc_s f xs [v] ::: (subst θ (s_ret S) :: Γ))
-| t_assign : 
-    forall Φ Γ v e τ φ, v <> ν ->
-      var_not_in v Γ -> expr_type Γ e { ν : τ | φ } ->
-(* ------------------------------------------------------------------- *)
-  (Φ / Γ ⊢ assign_s v e ::: ((v, { ν : τ | (var_e ν) .= e }) :: Γ))
-| t_seq : forall Φ Γ Γ' Γ'' s1 s2,
-  (Φ / Γ ⊢ s1 ::: Γ') -> (Φ / Γ' ⊢ s2 ::: Γ'') ->
-(* ------------------------------------------------------------------- *)
-  (Φ / Γ ⊢ seq_s s1 s2 ::: Γ'')
+  ((Φ ; Γ ; Ξ) ⊢ proc_s f xs [v] ::: (subst θ (s_ret S) :: Γ))
 
-where "P / G ⊢ s ::: O " := (stmt_type P G s O).
+| t_assign : 
+    forall Φ Γ Ξ v e τ φ, v <> ν ->
+      var_not_in v Γ -> expr_type Γ Ξ e { ν : τ | φ } ->
+(* ------------------------------------------------------------------- *)
+  ((Φ ; Γ ; Ξ)  ⊢ assign_s v e ::: ((v, { ν : τ | (var_e ν) .= e }) :: Γ))
+    
+| t_if : 
+    forall Φ Γ Γ1 Γ2 Γ' Ξ x s1 s2, 
+      ( Φ ; Γ ; ((var_e x) .= (int_v 1)) :: Ξ ) ⊢ s1 ::: Γ1 -> 
+      ( Φ ; Γ ; (not_r ((var_e x) .= (int_v 1))) :: Ξ) ⊢ s2 ::: Γ2 ->
+      join_env Ξ Γ1 Γ2 Γ' ->
+(* ------------------------------------------------------------------- *)
+  ((Φ ; Γ ; Ξ) ⊢ if_s x s1 s2 ::: Γ')
+
+| t_seq : forall Φ Ξ Γ Γ' Γ'' s1 s2,
+  (Φ ; Γ ; Ξ) ⊢ s1 ::: Γ' -> (Φ ; Γ' ; Ξ) ⊢ s2 ::: Γ'' ->
+(* ------------------------------------------------------------------- *)
+  ((Φ ; Γ ; Ξ) ⊢ seq_s s1 s2 ::: Γ'')
+
+where "( Φ ; Γ ; Ξ ) ⊢ s ::: O" := (stmt_type Φ Γ Ξ s O).
